Add dynamic indexing and static slicing to the netlist layer. (#155)

cava/cava/Cava/Monad/XilinxAdder.v
@@ -15,12 +15,18 @@
 
 From Coq Require Import Bool.Bool. 
 From Coq Require Import Ascii String.
+From Coq Require Import NArith.
+
+From Coq Require Import Vector.
+Import VectorNotations.
+
 From Coq Require Import Lists.List.
 Import ListNotations.
 
 Require Import ExtLib.Structures.Monads.
 
 Require Import Cava.Cava.
+Require Import Cava.VectorUtils.
 Require Import Cava.Monad.CavaMonad.
 
 Local Open Scope string_scope.
@@ -31,8 +37,11 @@ Local Open Scope type_scope.
 (* Build a full-adder with explicit use of Xilinx FPGA fast carry logic       *)
 (******************************************************************************)
 
-Definition xilinxFullAdder {m bit} `{Cava m bit} '(cin, (a, b))
+Definition xilinxFullAdder {m bit} `{Cava m bit}
+          (cin: bit)
+          (ab: bit * bit)
   : m (bit * bit)%type :=
+  let (a, b) := ab in
   part_sum <- xor2 (a, b) ;;
   sum <- xorcy (part_sum, cin) ;;
   cout <- muxcy part_sum cin a  ;;
@@ -41,7 +50,7 @@ Definition xilinxFullAdder {m bit} `{Cava m bit} '(cin, (a, b))
 (* A proof that the the full-adder is correct. *)
 Lemma xilinxFullAdder_behaviour :
   forall (a : bool) (b : bool) (cin : bool),
-         combinational (xilinxFullAdder (cin, (a, b)))
+         combinational (xilinxFullAdder cin (a, b))
          = (xorb cin (xorb a b),
            (a && b) || (b && cin) || (a && cin)).
 Proof.
@@ -57,16 +66,35 @@ Qed.
 (* An unsigned adder built using the fast carry full-adder.                   *)
 (******************************************************************************)
 
-Definition xilinxAdderWithCarry {m bit} `{Cava m bit} '(cin, (a, b))
-           : m (list bit * bit) 
-  := col xilinxFullAdder (cin, combine a b).
+Definition xilinxAdderWithCarry {m bit vec} `{Cava m bit vec} {n: nat}
+            (cinab : bit * (vec Bit (S n) * vec Bit (S n)))
+           : m (vec Bit (S n) * bit) 
+  := let '(cin, (a, b)) := cinab in
+     let aV : Vector.t bit (S n) := vecToVector1 a in
+     let bV : Vector.t bit (S n) := vecToVector1 b in
+     '(sum, cout) <- colV n xilinxFullAdder cin (vcombine aV bV) ;;
+     ret (vecBoolList sum, cout).
+
+(* A quick sanity check of the Xilinx adder with carry in and out *)
+Example xilinx_add_17_52:
+  combinational (xilinxAdderWithCarry
+                (false, (N2Bv_sized 8 17, N2Bv_sized 8 52))) =
+                (N2Bv_sized 8 69, false).
+Proof. reflexivity. Qed.                
 
 (******************************************************************************)
-(* An unsigned adder which does not have a carry-in and uses the carry-out    *)
-(* for bit-growth at the output.                   *)
+(* An unsigned adder with no bit-growth and no carry in                       *)
 (******************************************************************************)
 
-Definition xilinxAdder {m bit} `{Cava m bit} a b : m (list bit) :=
+Definition xilinxAdder {m bit vec} `{Cava m bit vec} {n: nat}
+            (a: vec Bit (S n)) (b: vec Bit (S n))
+           : m (vec Bit (S n)) :=
   z <- zero ;;
   '(sum, carry) <- xilinxAdderWithCarry (z, (a, b)) ;;
-  ret (sum ++ [carry]).
+  ret sum.
+
+(* A quick sanity check of the Xilinx adder with no bit-growth *)
+Example xilinx_no_growth_add_17_52:
+  combinational (xilinxAdder (N2Bv_sized 8 17) (N2Bv_sized 8 52)) =
+                 N2Bv_sized 8 69.
+Proof. reflexivity. Qed.
