cava/cava/Cava/Extraction.v
@@ -26,7 +26,9 @@ Set Extraction File Comment "Auto-generated from Cava/Coq. Please do not hand ed
 
 Require Import Cava.BitArithmetic.
 Require Import Cava.Cava.
+Require Import Cava.Kind.
 Require Import Cava.Signal.
+Require Import Cava.VectorUtils.
 Require Import Cava.Monad.CavaMonad.
 Require Import Cava.Monad.CombinationalMonad.
 Require Import Cava.Monad.CavaClass.
@@ -47,7 +49,7 @@ Require Import Cava.Arrow.Kappa.Kappa.
 Require Import Cava.Arrow.Kappa.CC.
 Require Import Cava.Arrow.Kappa.Syntax.
 Require Import Cava.Arrow.Instances.Combinational.
-Require Import Cava.Arrow.Instances.Netlist.
+(* Require Import Cava.Arrow.Instances.Netlist. *)
 Require Import Cava.Arrow.Instances.Constructive.
 Recursive Extraction Library Arrow.
 Recursive Extraction Library Kappa.
@@ -57,6 +59,8 @@ Recursive Extraction Library Constructive.
 
 Recursive Extraction Library Netlist.
 Recursive Extraction Library Signal.
+Recursive Extraction Library Kind.
 Recursive Extraction Library Types.
+Recursive Extraction Library VectorUtils.
 Recursive Extraction Library UnsignedAdders.
 Recursive Extraction Library XilinxAdder.
