cava/cava/Cava/VectorUtils.v
@@ -1,0 +1,139 @@
+(****************************************************************************)
+(* Copyright 2020 The Project Oak Authors                                   *)
+(*                                                                          *)
+(* Licensed under the Apache License, Version 2.0 (the "License")           *)
+(* you may not use this file except in compliance with the License.         *)
+(* You may obtain a copy of the License at                                  *)
+(*                                                                          *)
+(*     http://www.apache.org/licenses/LICENSE-2.0                           *)
+(*                                                                          *)
+(* Unless required by applicable law or agreed to in writing, software      *)
+(* distributed under the License is distributed on an "AS IS" BASIS,        *)
+(* WITHOUT WARRANTIES OR CONDITIONS OF ANY KIND, either express or implied. *)
+(* See the License for the specific language governing permissions and      *)
+(* limitations under the License.                                           *)
+(****************************************************************************)
+
+From Coq Require Import Lists.List.
+Import ListNotations.
+
+From Coq Require Import Vector.
+Import VectorNotations.
+
+Require Import Arith.
+
+From ExtLib Require Import Structures.Applicative.
+From ExtLib Require Import Structures.Traversable.
+Require Export ExtLib.Data.Monads.IdentityMonad.
+
+Section traversable.
+  Universe u v vF.
+  Context {F : Type@{v} -> Type@{vF}}.
+  Context {Applicative_F : Applicative F}.
+  Context {A : Type@{u}} {B : Type@{v}}.
+  Variable f : A -> F B.
+
+  Fixpoint mapT_vector@{} {n} (v : Vector.t A n ) : F (Vector.t B n).
+  Proof.
+    inversion v.
+    exact (@pure F _ _ []%vector).
+    refine (
+        let _1 := fun y ys => @Vector.cons B y _ ys in
+        let _2 := @pure F _ _ _1 in
+        let _3 := @ap F _ _ _ _2 (f h) in
+        let xs' := mapT_vector _ X in
+        let _4 := @ap F _ _ _  _3 in
+        _
+    ).
+    apply _4 in xs' .
+    exact xs'.
+  Defined.
+End traversable.
+
+Definition fixup n (F : Type -> Type) (Ap: Applicative F) (A B : Type) (m: A -> F B) := @mapT_vector F Ap A B m n.
+
+Global Instance Traversable_vector@{} {n} : Traversable (fun t => Vector.t t n) :=
+{ mapT := fixup n }.
+
+(******************************************************************************)
+(* Vector version of combine                                                  *)
+(******************************************************************************)
+
+Local Open Scope vector_scope.
+
+Fixpoint vcombine {A B: Type} {s: nat} (a: Vector.t A s) 
+                                       (b: Vector.t B s) :
+                                       Vector.t (A * B) s :=
+
+  match s, a, b with
+  | O, _, _ => []
+  | S n, a, b => let (x, xs) := Vector.uncons a in
+                 let (y, ys) := Vector.uncons b in
+                 (x, y) :: vcombine xs ys
+  end.
+
+Local Close Scope vector_scope.
+
+(* Vector version of seq *)
+
+Program Definition vseq (start len: nat) : Vector.t nat len :=
+  Vector.of_list (List.seq start len).
+Next Obligation.
+  rewrite List.seq_length. reflexivity.
+Defined.
+
+(* An experimental alternative vector representation *)
+
+Fixpoint AltVector (A: Type) (n: nat) : Type :=
+  match n with
+  | 0 => unit
+  | S m => (A * AltVector A m)%type
+  end.
+
+Definition v1 : AltVector nat 3 := (1, (2, (3, tt))).
+
+Fixpoint altVectorToList {A: Type} {n: nat} (v: AltVector A n) : list A :=
+  match n, v with
+  | 0, _ => []%list
+  | _, (x, v) => x :: altVectorToList v
+  end.
+
+Lemma vecConsFactL: forall (A: Type) (n: nat),
+      (A * AltVector A n)%type = AltVector A (n+1).
+Proof.
+  induction n.
+  - auto.
+  - simpl. rewrite IHn. reflexivity.
+Qed.
+
+Definition vecConsFact {A: Type} {n: nat} (v: A * AltVector A n) :
+                                              AltVector A (n+1).
+Proof.
+  induction n.
+  - auto.
+  - simpl. rewrite Nat.add_1_r. apply v.
+Qed.
+                                                
+Program Definition consAltVector {A: Type} {n: nat} (a: A) (v: AltVector A n) :
+                         AltVector A (n+1) :=
+   vecConsFact (a, v).
+
+Lemma length_cons: forall A (x:A) (xs: list A), length (x :: xs) = length xs + 1.
+Proof.
+  induction xs.
+  - simpl. reflexivity.
+  - simpl. rewrite <- IHxs. simpl. reflexivity.
+Qed.  
+
+Definition vec_cons {A} {x: A} {xs: list A} (v: AltVector A (length xs + 1)) :
+                    AltVector A (length (x :: xs)).
+Proof.
+  rewrite length_cons.
+  apply v.
+Qed.
+
+Fixpoint listToAltVector {A: Type} (l: list A) : AltVector A (length l) :=
+  match l return AltVector A (length l)  with
+  | [] => tt
+  | x::xs => vec_cons (consAltVector x (listToAltVector xs))
+  end.
